theories/LogicalRelation/Induction.v
@@ -1,6 +1,6 @@
 (** * LogRel.LogicalRelation.Induction: good induction principles for the logical relation. *)
 From LogRel.AutoSubst Require Import core unscoped Ast Extra.
-From LogRel Require Import Utils BasicAst Notations Context NormalForms Weakening UntypedReduction
+From LogRel Require Import Utils BasicAst Notations LContexts Context NormalForms Weakening UntypedReduction
 GenericTyping LogicalRelation.
 
 Set Universe Polymorphism.
@@ -27,17 +27,20 @@ Section Inductions.
 
 (** Reducibility at a lower level implies reducibility at a higher level, and their decoding are the
 same. Both need to be proven simultaneously, because of contravariance in the product case. *)
-
   Fixpoint LR_embedding@{i j k l} {l l'} (l_ : l << l')
-    {Γ A rEq rTe rTeEq} (lr : LogRel@{i j k l} l Γ A rEq rTe rTeEq) {struct lr} : (LogRel@{i j k l} l' Γ A rEq rTe rTeEq) :=
-    let embedΠad {Γ A} {ΠA : [Γ ||-Πd A]} (ΠAad : PiRedTyAdequate _ ΠA) :=
+    {wl Γ A rEq rTe rTeEq} (lr : LogRel@{i j k l} l wl Γ A rEq rTe rTeEq) {struct lr} :
+    (LogRel@{i j k l} l' wl Γ A rEq rTe rTeEq) :=
+    let embedΠad {wl Γ A} {ΠA : [Γ ||-Πd A]< wl >} (ΠAad : PiRedTyAdequate _ ΠA) :=
         {|
           PiRedTy.domAd :=
-            fun (Δ : context) (ρ : Δ ≤ _) (h : [  |- Δ]) => LR_embedding l_ (ΠAad.(PiRedTy.domAd) ρ h) ;
+            fun (Δ : context) wl' (ρ : Δ ≤ _) (τ : wl' ≤ε wl) Ninfl (h : [  |- Δ]< wl' >) => LR_embedding l_ (ΠAad.(PiRedTy.domAd) ρ τ Ninfl h) ;
           PiRedTy.codAd :=
-            fun (Δ : context) (a : term) (ρ : Δ ≤ _) (h : [  |- Δ])
-              (ha : [PiRedTy.domRed ΠA ρ h | Δ ||- a : _]) =>
-            LR_embedding l_ (ΠAad.(PiRedTy.codAd) ρ h ha)
+            fun (Δ : context) (wl' : wfLCon) (a : term)(ρ : Δ ≤ _) (τ : wl' ≤ε wl)
+                (Ninfl : _ <= length wl') (h : [ |- Δ ]< wl' >) 
+                (ha : [PiRedTy.domRed ΠA ρ τ Ninfl h | Δ ||- a : _]< wl' >)
+                wl'' (τ' : wl'' ≤ε wl')
+                (Minfl : _ <= length wl'')  =>
+            LR_embedding l_ (ΠAad.(PiRedTy.codAd) ρ τ Ninfl h ha τ' Minfl)
         |}
     in
     match lr with
@@ -48,154 +51,199 @@ same. Both need to be proven simultaneously, because of contravariance in the pr
     | LRne _ neA => LRne _ neA
     | LRPi _ ΠA ΠAad => LRPi _ ΠA (embedΠad ΠAad)
     | LRNat _ NA => LRNat _ NA
+    | LRBool _ NA => LRBool _ NA
     | LREmpty _ NA => LREmpty _ NA
     end.
 
   (** A basic induction principle, that handles only the first point in the list above *)
 
-  Notation PiHyp P Γ ΠA HAad G :=
-    ((forall {Δ} (ρ : Δ ≤ Γ) (h : [ |- Δ]),
-        P (HAad.(PiRedTy.domAd) ρ h)) ->
-      (forall {Δ a} (ρ : Δ ≤ Γ) (h : [ |- Δ ]) 
-        (ha : [ ΠA.(PiRedTy.domRed) ρ h | Δ ||- a : ΠA.(PiRedTy.dom)⟨ρ⟩ ]),
-        P (HAad.(PiRedTy.codAd) ρ h ha)) -> G).
-
+  Notation PiHyp P wl Γ ΠA HAad G :=
+    ((forall {Δ wl'} (ρ : Δ ≤ Γ) (τ : wl' ≤ε wl)
+             (Ninfl : _ <= length wl')
+             (h : [ |- Δ]< wl' >),
+        P (HAad.(PiRedTy.domAd) ρ τ Ninfl h)) ->
+     (forall {Δ wl' a} (ρ : Δ ≤ Γ) (τ : wl' ≤ε wl)
+             (Ninfl : _ <= length wl')
+             (h : [ |- Δ ]< wl' >) 
+             (ha : [ ΠA.(PiRedTy.domRed) ρ τ Ninfl h | Δ ||- a : ΠA.(PiRedTy.dom)⟨ρ⟩ ]< wl' >)
+             {wl''} (τ' : wl'' ≤ε wl')
+             (Minfl : _ <= length wl''),
+         P (HAad.(PiRedTy.codAd) ρ τ Ninfl h ha τ' Minfl)) -> G).
+        
   Theorem LR_rect@{i j k o}
     (l : TypeLevel)
     (rec : forall l', l' << l -> RedRel@{i j})
-    (P : forall {c t rEq rTe rTeEq},
-      LR@{i j k} rec c t rEq rTe rTeEq  -> Type@{o}) :
+    (P : forall {wl c t rEq rTe rTeEq},
+      LR@{i j k} rec wl c t rEq rTe rTeEq  -> Type@{o}) :
 
-    (forall (Γ : context) A (h : [Γ ||-U<l> A]),
+    (forall (wl : wfLCon) (Γ : context) A (h : [Γ ||-U<l> A]< wl >),
       P (LRU rec h)) ->
 
-    (forall (Γ : context) (A : term) (neA : [Γ ||-ne A]),
+    (forall (wl : wfLCon) (Γ : context) (A : term) (neA : [Γ ||-ne A]< wl >),
       P (LRne rec neA)) -> 
 
-    (forall (Γ : context) (A : term) (ΠA : PiRedTy@{j} Γ A) (HAad : PiRedTyAdequate (LR rec) ΠA),
-      PiHyp P Γ ΠA HAad (P (LRPi rec ΠA HAad))) ->
+    (forall (wl : wfLCon) (Γ : context) (A : term)
+            (ΠA : PiRedTy@{j} wl Γ A) (HAad : PiRedTyAdequate (LR rec) ΠA),
+      PiHyp P wl Γ ΠA HAad (P (LRPi rec ΠA HAad))) ->
 
-    (forall Γ A (NA : [Γ ||-Nat A]), P (LRNat rec NA)) ->
+    (forall wl Γ A (NA : [Γ ||-Nat A]< wl >), P (LRNat rec NA)) ->
 
-    (forall Γ A (NA : [Γ ||-Empty A]), P (LREmpty rec NA)) ->
+    (forall wl Γ A (NA : [Γ ||-Bool A]< wl >), P (LRBool rec NA)) ->
+    
+    (forall wl Γ A (NA : [Γ ||-Empty A]< wl >), P (LREmpty rec NA)) ->
 
-    forall (Γ : context) (t : term) (rEq rTe : term -> Type@{j})
-      (rTeEq  : term -> term -> Type@{j}) (lr : LR@{i j k} rec Γ t rEq rTe rTeEq),
+    forall (wl : wfLCon) (Γ : context) (t : term) (rEq rTe : term -> Type@{j})
+           (rTeEq  : term -> term -> Type@{j})
+           (lr : LR@{i j k} rec wl Γ t rEq rTe rTeEq),
       P lr.
   Proof.
     cbn.
-    intros HU Hne HPi HNat HEmpty.
-    fix HRec 6.
+    intros HU Hne HPi HNat HBool HEmpty.
+    fix HRec 7.
     destruct lr.
     - eapply HU.
     - eapply Hne.
     - eapply HPi.
       all: intros ; eapply HRec.
     - eapply HNat.
+    - eapply HBool.
     - eapply HEmpty.
   Defined.
 
   Definition LR_rec@{i j k} := LR_rect@{i j k Set}.
   
-  Notation PiHypLogRel P Γ ΠA G :=
-    ((forall {Δ} (ρ : Δ ≤ Γ) (h : [ |- Δ]), P (ΠA.(PiRedTyPack.domRed) ρ h).(LRAd.adequate)) ->
-    (forall {Δ a} (ρ : Δ ≤ Γ) (h : [ |- Δ ]) 
-      (ha : [ Δ ||-< _ > a : ΠA.(PiRedTyPack.dom)⟨ρ⟩ |  ΠA.(PiRedTyPack.domRed) ρ h ]),
-      P (ΠA.(PiRedTyPack.codRed) ρ h ha).(LRAd.adequate)) -> G).
+  Notation PiHypLogRel P wl Γ ΠA G :=
+    ((forall {Δ wl'} (ρ : Δ ≤ Γ) (τ : wl' ≤ε wl)
+             (Ninfl : _ <= length wl')
+             (h : [ |- Δ]< wl' >),
+         P (ΠA.(PiRedTyPack.domRed) ρ τ Ninfl h).(LRAd.adequate)) ->
+    (forall {Δ wl' a} (ρ : Δ ≤ Γ) (τ : wl' ≤ε wl)
+             (Ninfl : _ <= length wl')
+             (h : [ |- Δ ]< wl' >) 
+             (ha : [ Δ ||-< _ > a : ΠA.(PiRedTyPack.dom)⟨ρ⟩ |  ΠA.(PiRedTyPack.domRed) ρ τ Ninfl h ]< wl' >)
+             {wl''} (τ' : wl'' ≤ε wl')
+             (Minfl : _ <= length wl''),
+        P (ΠA.(PiRedTyPack.codRed) ρ τ Ninfl h ha τ' Minfl).(LRAd.adequate)) -> G).
 
 
   (** Induction principle specialized to LogRel as the reducibility relation on lower levels *)
   Theorem LR_rect_LogRelRec@{i j k l o}
-    (P : forall {l Γ t rEq rTe rTeEq},
-    LogRel@{i j k l} l Γ t rEq rTe rTeEq -> Type@{o}) :
+    (P : forall {l wl Γ t rEq rTe rTeEq},
+    LogRel@{i j k l} l wl Γ t rEq rTe rTeEq -> Type@{o}) :
 
-    (forall l (Γ : context) A (h : [Γ ||-U<l> A]),
+    (forall l (wl : wfLCon) (Γ : context) A (h : [Γ ||-U<l> A]< wl >),
       P (LRU (LogRelRec l) h)) ->
 
-    (forall (l : TypeLevel) (Γ : context) (A : term) (neA : [Γ ||-ne A]),
+    (forall (l : TypeLevel) (wl : wfLCon) (Γ : context) (A : term)
+            (neA : [Γ ||-ne A]< wl >),
       P (LRne (LogRelRec l) neA)) ->
 
-    (forall (l : TypeLevel) (Γ : context) (A : term) (ΠA : PiRedTyPack@{i j k l} Γ A l),
-      PiHypLogRel P Γ ΠA (P (LRPi' ΠA).(LRAd.adequate ))) ->
+    (forall (l : TypeLevel) (wl : wfLCon) (Γ : context) (A : term)
+            (ΠA : PiRedTyPack@{i j k l} wl Γ A l),
+      PiHypLogRel P wl Γ ΠA (P (LRPi' ΠA).(LRAd.adequate ))) ->
     
-    (forall l Γ A (NA : [Γ ||-Nat A]), P (LRNat (LogRelRec l) NA)) ->
+    (forall l wl Γ A (NA : [Γ ||-Nat A]< wl >), P (LRNat (LogRelRec l) NA)) ->
+    
+    (forall l wl Γ A (NA : [Γ ||-Bool A]< wl >), P (LRBool (LogRelRec l) NA)) ->
 
-    (forall l Γ A (NA : [Γ ||-Empty A]), P (LREmpty (LogRelRec l) NA)) ->
+    (forall l wl Γ A (NA : [Γ ||-Empty A]< wl >), P (LREmpty (LogRelRec l) NA)) ->
 
-    forall (l : TypeLevel) (Γ : context) (t : term) (rEq rTe : term -> Type@{k})
-      (rTeEq  : term -> term -> Type@{k}) (lr : LR@{j k l} (LogRelRec@{i j k} l) Γ t rEq rTe rTeEq),
+    forall (l : TypeLevel) (wl : wfLCon) (Γ : context) (t : term)
+           (rEq rTe : term -> Type@{k})
+           (rTeEq  : term -> term -> Type@{k})
+           (lr : LR@{j k l} (LogRelRec@{i j k} l) wl Γ t rEq rTe rTeEq),
       P lr.
   Proof.
     intros HU Hne HPi **; eapply LR_rect@{j k l o}.
-    1,2,4,5: auto.
-    - intros; eapply (HPi _ _ _ (PiRedTyPack.pack ΠA HAad)); eauto.
+    1,2,4,5,6: auto.
+    - intros; eapply (HPi _ _ _ _ (PiRedTyPack.pack ΠA HAad)); eauto.
   Defined.
 
 
   Theorem LR_rect_TyUr@{i j k l o}
-    (P : forall {l Γ A}, [LogRel@{i j k l} l | Γ ||- A] -> Type@{o}) :
+    (P : forall {l wl Γ A}, [LogRel@{i j k l} l | Γ ||- A]< wl > -> Type@{o}) :
 
-    (forall l (Γ : context) A (h : [Γ ||-U<l> A]),
+    (forall l wl (Γ : context) A (h : [Γ ||-U<l> A]< wl >),
       P (LRU_ h)) ->
 
-    (forall (l : TypeLevel) (Γ : context) (A : term) (neA : [Γ ||-ne A]),
+    (forall (l : TypeLevel) wl (Γ : context) (A : term) (neA : [Γ ||-ne A]< wl >),
       P (LRne_ l neA)) ->
 
-    (forall (l : TypeLevel) (Γ : context) (A : term) (ΠA : PiRedTyPack@{i j k l} Γ A l),
-      (forall {Δ} (ρ : Δ ≤ Γ) (h : [ |- Δ]), P (ΠA.(PiRedTyPack.domRed) ρ h)) ->
-      (forall {Δ a} (ρ : Δ ≤ Γ) (h : [ |- Δ ]) 
-       (ha : [ ΠA.(PiRedTyPack.domRed) ρ h | Δ ||- a : ΠA.(PiRedTyPack.dom)⟨ρ⟩ ]),
-      P (ΠA.(PiRedTyPack.codRed) ρ h ha)) ->
-    P (LRPi' ΠA)) ->
+    (forall (l : TypeLevel) wl (Γ : context) (A : term)
+            (ΠA : PiRedTyPack@{i j k l} wl Γ A l),
+        (forall {Δ wl'} (ρ : Δ ≤ Γ) (τ : wl' ≤ε wl)
+             (Ninfl : _ <= length wl')
+             (h : [ |- Δ ]< wl' >),
+            P (ΠA.(PiRedTyPack.domRed) ρ τ Ninfl h)) ->
+        (forall {Δ wl' a} (ρ : Δ ≤ Γ) (τ : wl' ≤ε wl)
+             (Ninfl : _ <= length wl')
+             (h : [ |- Δ ]< wl' >)
+             (ha : [ ΠA.(PiRedTyPack.domRed) ρ τ Ninfl h | Δ ||- a : ΠA.(PiRedTyPack.dom)⟨ρ⟩ ]< wl' >) {wl''} (τ' : wl'' ≤ε wl')
+             (Minfl : _ <= length wl''),
+            P (ΠA.(PiRedTyPack.codRed) ρ τ Ninfl h ha τ' Minfl)) ->
+        P (LRPi' ΠA)) ->
 
-    (forall l Γ A (NA : [Γ ||-Nat A]), P (LRNat_ l NA)) ->
+    (forall l wl Γ A (NA : [Γ ||-Nat A]< wl >), P (LRNat_ l NA)) ->
+    
+    (forall l wl Γ A (NA : [Γ ||-Bool A]< wl >), P (LRBool_ l NA)) ->
 
-    (forall l Γ A (NA : [Γ ||-Empty A]), P (LREmpty_ l NA)) ->
+    (forall l wl Γ A (NA : [Γ ||-Empty A]< wl >), P (LREmpty_ l NA)) ->
 
-    forall (l : TypeLevel) (Γ : context) (A : term) (lr : [LogRel@{i j k l} l | Γ ||- A]),
+    forall (l : TypeLevel) wl (Γ : context) (A : term)
+           (lr : [LogRel@{i j k l} l | Γ ||- A]< wl >),
       P lr.
   Proof.
-    intros HU Hne HPi HNat HEmpty l Γ A lr.
-    apply (LR_rect_LogRelRec@{i j k l o} (fun l Γ A _ _ _ lr => P l Γ A (LRbuild lr))).
+    intros HU Hne HPi HNat HBool HEmpty l wl Γ A lr.
+    apply (LR_rect_LogRelRec@{i j k l o} (fun l wl Γ A _ _ _ lr => P l wl Γ A (LRbuild lr))).
     all: auto.
   Defined.
 
-  Notation PiHyp0 P Γ ΠA HAad G :=
-    ((forall {Δ} (ρ : Δ ≤ Γ) (h : [ |- Δ]),
-        P (HAad.(PiRedTy.domAd) ρ h)) ->
-      (forall {Δ a} (ρ : Δ ≤ Γ) (h : [ |- Δ ]) 
-        (ha : [ ΠA.(PiRedTy.domRed) ρ h | Δ ||- a : ΠA.(PiRedTy.dom)⟨ρ⟩ ]),
-        P (HAad.(PiRedTy.codAd) ρ h ha)) -> G).
+  Notation PiHyp0 wl P Γ ΠA HAad G :=
+    ((forall {Δ wl'} (ρ : Δ ≤ Γ) (τ : wl' ≤ε wl)
+             (Ninfl : _ <= length wl')
+             (h : [ |- Δ]< wl' >),
+         P (HAad.(PiRedTy.domAd) ρ τ Ninfl h)) ->
+      (forall {Δ wl' a} (ρ : Δ ≤ Γ) (τ : wl' ≤ε wl)
+              (Ninfl : _ <= length wl')
+              (h : [ |- Δ ]< wl' >) 
+              (ha : [ ΠA.(PiRedTy.domRed) ρ τ Ninfl h | Δ ||- a : ΠA.(PiRedTy.dom)⟨ρ⟩ ]< wl' >)
+             {wl''} (τ' : wl'' ≤ε wl')
+             (Minfl : _ <= length wl''),
+        P (HAad.(PiRedTy.codAd) ρ τ Ninfl h ha τ' Minfl)) -> G).
 
+  
 
   (** Induction principle specialized at level 0 to minimize universe constraints. *)
   (* Useful anywhere ? *)
   Theorem LR_rect0@{i j k o}
-    (P : forall {c t rEq rTe rTeEq},
-      LogRel0@{i j k} c t rEq rTe rTeEq  -> Type@{o}) :
+    (P : forall {wl c t rEq rTe rTeEq},
+      LogRel0@{i j k} wl c t rEq rTe rTeEq  -> Type@{o}) :
 
-    (forall (Γ : context) (A : term) (neA : [Γ ||-ne A]),
+    (forall wl (Γ : context) (A : term) (neA : [Γ ||-ne A]< wl >),
       P (LRne rec0 neA)) -> 
     
-    (forall (Γ : context) (A : term) (ΠA : PiRedTy@{j} Γ A) (HAad : PiRedTyAdequate LogRel0@{i j k} ΠA),
-      PiHyp0 P Γ ΠA HAad (P (LRPi rec0 ΠA HAad))) ->
+    (forall wl (Γ : context) (A : term) (ΠA : PiRedTy@{j} wl Γ A) (HAad : PiRedTyAdequate LogRel0@{i j k} ΠA),
+      PiHyp0 wl P Γ ΠA HAad (P (LRPi rec0 ΠA HAad))) ->
 
-    (forall Γ A (NA : [Γ ||-Nat A]), P (LRNat rec0 NA)) ->
+    (forall wl Γ A (NA : [Γ ||-Nat A]< wl >), P (LRNat rec0 NA)) ->
+    
+    (forall wl Γ A (NA : [Γ ||-Bool A]< wl >), P (LRBool rec0 NA)) ->
 
-    (forall Γ A (NA : [Γ ||-Empty A]), P (LREmpty rec0 NA)) ->
+    (forall wl Γ A (NA : [Γ ||-Empty A]< wl >), P (LREmpty rec0 NA)) ->
 
-    forall (Γ : context) (t : term) (rEq rTe : term -> Type@{j})
-      (rTeEq  : term -> term -> Type@{j}) (lr : LogRel0@{i j k} Γ t rEq rTe rTeEq),
+    forall wl (Γ : context) (t : term) (rEq rTe : term -> Type@{j})
+      (rTeEq  : term -> term -> Type@{j}) (lr : LogRel0@{i j k} wl Γ t rEq rTe rTeEq),
       P lr.
   Proof.
     cbn.
-    intros Hne HPi HNat HEmpty.
-    fix HRec 6.
+    intros Hne HPi HNat HBool HEmpty.
+    fix HRec 7.
     destruct lr.
     - destruct H as [? lt]; destruct (elim lt).
     - eapply Hne.
     - eapply HPi; intros ; eapply HRec.
     - eapply HNat.
+    - eapply HBool.
     - eapply HEmpty.
   Defined.
 
@@ -210,17 +258,19 @@ Section Inversions.
     `{!RedType ta} `{!TypeNf ta} `{!TypeNe ta} `{!RedTerm ta} `{!TermNf ta} `{!TermNe ta} `{!RedTypeProperties}
     `{!TypeNeProperties}.
 
-  Lemma invLR {Γ l A A'} (lr : [Γ ||-<l> A]) (r : [A ⇒* A']) (w : isType A') :
+  Lemma invLR {wl Γ l A A'}
+    (lr : [Γ ||-<l> A]< wl >) (r : [A ⇒* A']< wl >) (w : isType wl A') :
     match w return Type with
-    | UnivType => [Γ ||-U<l> A]
-    | ProdType => [Γ ||-Π<l> A]
-    | NatType => [Γ ||-Nat A]
-    | EmptyType => [Γ ||-Empty A]
-    | NeType _ => [Γ ||-ne A]
+    | UnivType _ => [Γ ||-U<l> A]< wl >
+    | ProdType _ => [Γ ||-Π<l> A]< wl >
+    | NatType _ => [Γ ||-Nat A]< wl >
+    | BoolType _ => [Γ ||-Bool A]< wl >
+    | EmptyType _ => [Γ ||-Empty A]< wl >
+    | NeType _ _ => [Γ ||-ne A]< wl >
     end.
   Proof.
     revert A' r w.
-    pattern l, Γ, A, lr ; eapply LR_rect_TyUr; clear l Γ A lr.
+    pattern l, wl, Γ, A, lr ; eapply LR_rect_TyUr; clear l wl Γ A lr.
     - intros * h ? red whA.
       assert (A' = U) as ->.
       {
@@ -233,7 +283,7 @@ Section Inversions.
       exfalso.
       gen_typing.
     - intros * ? A' red whA.
-      enough ({w' & whA = NeType w'}) as [? ->] by easy.
+      enough ({w' & whA = NeType _ w'}) as [? ->] by easy.
       destruct neA as [A'' redA neA''].
       apply ty_ne_whne in neA''.
       assert (A' = A'') as <-.
@@ -243,7 +293,7 @@ Section Inversions.
       + dependent inversion whA ; subst.
         all: inv_whne.
         all: now eexists.
-    - intros ??? PiA _ _ A' red whA.
+    - intros ???? PiA _ _ A' red whA.
       enough (∑ dom cod, A' = tProd cod dom) as (?&?&->).
       + dependent inversion whA ; subst.
         2: exfalso ; gen_typing.
@@ -253,14 +303,21 @@ Section Inversions.
         eapply whred_det.
         1-3: gen_typing.
         eapply redty_red, redA.
-    - intros ??? [redA] ???.
+    - intros ???? [redA] ???.
       enough (A' = tNat) as ->.
       + dependent inversion w. 
         1: now econstructor.
         inv_whne.
       + eapply whred_det; tea.
         all: gen_typing.
-    - intros ??? [redA] ???.
+    - intros ???? [redA] ???.
+      enough (A' = tBool) as ->.
+      + dependent inversion w. 
+        1: now econstructor.
+        inv_whne.
+      + eapply whred_det; tea.
+        all: gen_typing.
+    - intros ???? [redA] ???.
       enough (A' = tEmpty) as ->.
       + dependent inversion w. 
         1: now econstructor.
@@ -269,22 +326,22 @@ Section Inversions.
         all: gen_typing.
   Qed.
 
-  Lemma invLRU {Γ l} : [Γ ||-<l> U] -> [Γ ||-U<l> U].
+  Lemma invLRU {wl Γ l} : [Γ ||-<l> U]< wl > -> [Γ ||-U<l> U]< wl >.
   Proof.
     intros.
-    now unshelve eapply (invLR _ redIdAlg UnivType).
+    now unshelve eapply (invLR _ redIdAlg (UnivType wl)).
   Qed.
 
-  Lemma invLRne {Γ l A} : whne A -> [Γ ||-<l> A] -> [Γ ||-ne A].
+  Lemma invLRne {wl Γ l A} : whne wl A -> [Γ ||-<l> A]< wl > -> [Γ ||-ne A]< wl >.
   Proof.
     intros.
-    now unshelve eapply  (invLR _ redIdAlg (NeType _)).
+    now unshelve eapply  (invLR _ redIdAlg (NeType _ _)).
   Qed.
 
-  Lemma invLRΠ {Γ l dom cod} : [Γ ||-<l> tProd dom cod] -> [Γ ||-Π<l> tProd dom cod].
+  Lemma invLRΠ {wl Γ l dom cod} : [Γ ||-<l> tProd dom cod]< wl > -> [Γ ||-Π<l> tProd dom cod]< wl >.
   Proof.
     intros.
-    now unshelve eapply  (invLR _ redIdAlg ProdType).
+    now unshelve eapply  (invLR _ redIdAlg (ProdType _)).
   Qed.
 
   (* invLRNat is useless *)
